wip

Matroid/ForMathlib/Graph/Walk.lean
@@ -1,33 +1,32 @@
 import Matroid.ForMathlib.Graph.Basic
-import Mathlib.Data.List.Basic
+import Mathlib.Data.Set.Insert
 
-open Function Set List
+open Set Function List Nat
 
-variable {α β : Type*} {e e' f : β} {x y z u v : α} {G : Graph α β}
+variable {α β : Type*} {G H : Graph α β} {u v x y z : α} {e e' f g : β} {S S' T T' U V : Set α}
+  {F F' R R': Set β}
+
+namespace Graph
+
 
 inductive Walk (α β : Type*) where
 | nil (u : α) : Walk α β
 | cons (u : α) (e : β) (W : Walk α β) : Walk α β
 
-namespace Walk
 variable {w w₁ w₂ : Walk α β}
+namespace Walk
 
 def Nonempty : Walk α β → Prop
 | nil _ => False
 | cons _ _ _ => True
 
-def start : Walk α β → α
+def first : Walk α β → α
 | nil x => x
 | cons x _ _ => x
 
-def finish : Walk α β → α
+def last : Walk α β → α
 | nil x => x
-| cons _ _ w => w.finish
-
-def ValidIn (w : Walk α β) (G : Graph α β) : Prop :=
-  match w with
-  | nil x => x ∈ G.V
-  | cons x e w => G.Inc₂ e x w.start ∧ w.ValidIn G
+| cons _ _ w => w.last
 
 def vx : Walk α β → List α
 | nil x => [x]
@@ -41,90 +40,166 @@ instance [DecidableEq α] : Decidable (x ∈ w) := by
   infer_instance
 
 @[simp]
-lemma mem_iff : (x ∈ w) = (x ∈ w.vx) := rfl
+lemma mem_notation : (x ∈ w.vx) = (x ∈ w) := rfl
+
+def vxSet : Walk α β → Set α := fun w => {x | x ∈ w}
 
 def edge : Walk α β → List β
 | nil _ => []
 | cons _ e w => e :: w.edge
 
+def edgeSet : Walk α β → Set β := fun w => {e | e ∈ w.edge}
+
 def length : Walk α β → ℕ
 | nil _ => 0
 | cons _ _ w => w.length + 1
 
-def concat : Walk α β → β → α → Walk α β
-| nil x, e, y => cons x e (nil y)
-| cons x e w, f, y => cons x e (w.concat f y)
-
-def dropLast : Walk α β → Walk α β
-| nil x => nil x
-| cons x _ (nil _) => nil x
-| cons x e (cons y e' w) => cons x e ((cons y e' w).dropLast)
-
-/-- Append one walk `w` to another walk `w'` by replacing the last vertex of `w` with the walk `w'`.
-(Intended for the case where `w.last = w'.first`; the last vertex of `w` is ignored)  -/
-def append : Walk α β → Walk α β → Walk α β
-| nil _x, w => w
-| cons x e w, w' => cons x e (w.append w')
-
-instance instAppend : Append (Walk α β) where
-  append := append
-
-def IsPrefix : Walk α β → Walk α β → Prop :=
-  fun W w => ∃ w', W = w ++ w'
-
-def IsSuffix : Walk α β → Walk α β → Prop :=
-  fun W w => ∃ w', W = w' ++ w
-
-def reverse : Walk α β → Walk α β
-| nil x => nil x
-| cons x e w => w.reverse.concat e x
-
-def startAt [DecidableEq α] (w : Walk α β) (u : α) (h : u ∈ w) : Walk α β :=
+def ValidIn (w : Walk α β) (G : Graph α β) : Prop :=
   match w with
-  | nil x => nil x
-  | cons x e w =>
-    if hin : u ∈ w
-    then startAt w u hin
-    else cons x e w
+  | nil x => x ∈ G.V
+  | cons x e w => G.Inc₂ e x w.first ∧ w.ValidIn G
 
-@[simp]
-lemma cons_length : (cons x e w).length = w.length + 1 := rfl
+end Walk
 
-lemma startAt_length_le [DecidableEq α] {w : Walk α β} (h : u ∈ w) :
-    (startAt w u h).length ≤ w.length := by
-  match w with
-  | nil x => simp [startAt]
-  | cons x e w =>
-    simp only [startAt, cons_length]
-    split_ifs with hin
-    · have := startAt_length_le hin
-      omega
-    · simp
+@[mk_iff]
+structure IsTrail (G : Graph α β) (W : Walk α β) : Prop where
+  validIn : W.ValidIn G
+  edge_nodup : W.edge.Nodup
 
-def dedup [DecidableEq α] : Walk α β → Walk α β
-| nil x => nil x
-| cons x e w =>
-  if h : x ∈ w
-  then by
-    have := startAt_length_le h
-    exact (startAt w x h).dedup
-  else cons x e (dedup w)
-termination_by w => w.length
+@[simp] lemma IsTrail.validIn_simp (h : G.IsTrail w) : w.ValidIn G := h.validIn
+@[simp] lemma IsTrail.edge_nodup_simp (h : G.IsTrail w) : w.edge.Nodup := h.edge_nodup
+@[simp] lemma isTrail_simp (hVd : w.ValidIn G) (hed : w.edge.Nodup) :
+    G.IsTrail w := IsTrail.mk hVd hed
 
-@[simp] lemma cons_vx : (cons x e w).vx = x :: w.vx := rfl
+@[mk_iff]
+structure IsPath (G : Graph α β) (W : Walk α β) : Prop where
+  validIn : W.ValidIn G
+  nodup : W.vx.Nodup
+
+@[simp] lemma IsPath.validIn_simp (h : G.IsPath w) : w.ValidIn G := h.validIn
+@[simp] lemma IsPath.nodup_simp (h : G.IsPath w) : w.vx.Nodup := h.nodup
+@[simp] lemma isPath_simp (hVd : w.ValidIn G) (hnodup : w.vx.Nodup) :
+    G.IsPath w := IsPath.mk hVd hnodup
+
+@[mk_iff]
+structure IsWalkFrom (G : Graph α β) (S T : Set α) (W : Walk α β) : Prop where
+  validIn : W.ValidIn G
+  first_mem : W.first ∈ S
+  last_mem : W.last ∈ T
+
+@[simp] lemma IsWalkFrom.validIn_simp (h : G.IsWalkFrom S T w) : w.ValidIn G := h.validIn
+@[simp] lemma IsWalkFrom.first_mem_simp (h : G.IsWalkFrom S T w) : w.first ∈ S := h.first_mem
+@[simp] lemma IsWalkFrom.last_mem_simp (h : G.IsWalkFrom S T w) : w.last ∈ T := h.last_mem
+@[simp] lemma isWalkFrom_simp (hVd : w.ValidIn G) (hfirst : w.first ∈ S) (hlast : w.last ∈ T) :
+    G.IsWalkFrom S T w := IsWalkFrom.mk hVd hfirst hlast
+
+@[mk_iff]
+structure IsTrailFrom (G : Graph α β) (S T : Set α) (W : Walk α β) : Prop extends
+  G.IsTrail W, G.IsWalkFrom S T W
+
+@[mk_iff]
+structure IsPathFrom (G : Graph α β) (S T : Set α) (W : Walk α β) : Prop extends
+  G.IsPath W, G.IsWalkFrom S T W
+
+
+-- def IsClosed (W : Walk α β) : Prop := W.first = W.last
+
+@[mk_iff]
+structure IsCycle (G : Graph α β) (W : Walk α β) : Prop where
+  validIn : W.ValidIn G
+  nodup' : W.vx.dropLast.Nodup
+  closed : W.first = W.last
+
+@[simp] lemma isCycle_simp (hVd : w.ValidIn G) (hnodup : w.vx.dropLast.Nodup)
+    (hclosed : w.first = w.last) : G.IsCycle w := IsCycle.mk hVd hnodup hclosed
+
+
+/- Properties between IsWalkFrom, IsTrail, IsPath, IsTrailFrom, IsPathFrom -/
+
+-- lemma IsPath.isTrail (h : G.IsPath w) : G.IsTrail w where
+--   validIn := h.validIn
+--   edge_nodup := by
+--     _
+
+-- lemma IsCycle.isTrail (h : G.IsCycle w) : G.IsTrail w where
+--   validIn := h.validIn
+--   edge_nodup := sorry
+
+lemma IsTrailFrom.isTrail (h : G.IsTrailFrom S T w) : G.IsTrail w where
+  validIn := h.validIn
+  edge_nodup := h.edge_nodup
+
+lemma IsTrailFrom.isWalkFrom (h : G.IsTrailFrom S T w) : G.IsWalkFrom S T w where
+  validIn := h.validIn
+  first_mem := h.first_mem
+  last_mem := h.last_mem
+
+lemma IsPathFrom.isPath (h : G.IsPathFrom S T w) : G.IsPath w where
+  validIn := h.validIn
+  nodup := h.nodup
+
+lemma IsPathFrom.isWalkFrom (h : G.IsPathFrom S T w) : G.IsWalkFrom S T w where
+  validIn := h.validIn
+  first_mem := h.first_mem
+  last_mem := h.last_mem
+
+-- lemma IsPathFrom.isTrailFrom (h : G.IsPathFrom S T w) : G.IsTrailFrom S T w where
+--   validIn := h.validIn
+--   edge_nodup := h.isPath.isTrail.edge_nodup
+--   first_mem := h.first_mem
+--   last_mem := h.last_mem
+
+lemma Walk.ValidIn.isTrail (hVd : w.ValidIn G) (hedge : w.edge.Nodup) : G.IsTrail w := ⟨hVd, hedge⟩
+
+lemma Walk.ValidIn.isPath (hVd : w.ValidIn G) (hvx : w.vx.Nodup) : G.IsPath w := ⟨hVd, hvx⟩
+
+lemma Walk.ValidIn.isWalkFrom (hVd : w.ValidIn G) (hfirst : w.first ∈ S) (hlast : w.last ∈ T) :
+    G.IsWalkFrom S T w := ⟨hVd, hfirst, hlast⟩
+
+lemma Walk.ValidIn.isCycle (hVd : w.ValidIn G) (hvx : w.vx.dropLast.Nodup)
+    (hclosed : w.first = w.last) : G.IsCycle w := ⟨hVd, hvx, hclosed⟩
+
+lemma Walk.ValidIn.isTrailFrom (hVd : w.ValidIn G) (hedge : w.edge.Nodup) (hfirst : w.first ∈ S)
+    (hlast : w.last ∈ T) : G.IsTrailFrom S T w := ⟨⟨hVd, hedge⟩, hfirst, hlast⟩
+
+lemma Walk.ValidIn.isPathFrom (hVd : w.ValidIn G) (hvx : w.vx.Nodup) (hfirst : w.first ∈ S)
+    (hlast : w.last ∈ T) : G.IsPathFrom S T w := ⟨⟨hVd, hvx⟩, hfirst, hlast⟩
+
+lemma IsTrail.isPath (hT : G.IsTrail w) (hvx : w.vx.Nodup) : G.IsPath w := ⟨hT.validIn, hvx⟩
+
+lemma IsTrail.isCycle (hT : G.IsTrail w) (hvx : w.vx.dropLast.Nodup) (hclosed : w.first = w.last) :
+    G.IsCycle w := ⟨hT.validIn, hvx, hclosed⟩
+
+lemma IsTrail.isTrailFrom (hT : G.IsTrail w) (hfirst : w.first ∈ S) (hlast : w.last ∈ T) :
+    G.IsTrailFrom S T w := ⟨hT, hfirst, hlast⟩
+
+lemma IsTrail.isPathFrom (hT : G.IsTrail w) (hvx : w.vx.Nodup) (hfirst : w.first ∈ S)
+    (hlast : w.last ∈ T) : G.IsPathFrom S T w := ⟨⟨hT.validIn, hvx⟩, hfirst, hlast⟩
+
+lemma IsPath.isPathFrom (hP : G.IsPath w) (hfirst : w.first ∈ S) (hlast : w.last ∈ T) :
+    G.IsPathFrom S T w := ⟨hP, hfirst, hlast⟩
+
+namespace Walk
+
+/- Properties of nil -/
+
+@[simp] lemma nil_not_nonempty : ¬ (nil x : Walk α β).Nonempty := by simp [Nonempty]
+
+@[simp] lemma nil_first : (nil x : Walk α β).first = x := rfl
+
+@[simp] lemma nil_last : (nil x : Walk α β).last = x := rfl
 
 @[simp] lemma nil_vx : (nil x : Walk α β).vx = [x] := rfl
 
+@[simp] lemma mem_nil_iff : x ∈ (nil u : Walk α β) ↔ x = u := by simp [← mem_notation]
+
+@[simp] lemma nil_vxSet : (nil x : Walk α β).vxSet = {x} := by simp [vxSet]
+
 @[simp] lemma nil_edge : (nil x : Walk α β).edge = [] := rfl
 
+@[simp] lemma nil_edgeSet : (nil x : Walk α β).edgeSet = ∅ := by simp [edgeSet]
+
 @[simp] lemma nil_length : (nil x : Walk α β).length = 0 := rfl
-
-@[simp] lemma nil_start : (nil x : Walk α β).start = x := rfl
-
-@[simp] lemma nil_finish : (nil x : Walk α β).finish = x := rfl
-
-@[simp] lemma nil_ValidIn_iff : (nil x : Walk α β).ValidIn G ↔ x ∈ G.V := by
-  simp only [ValidIn]
 
 @[simp] lemma nil_injective : Injective (nil : α → Walk α β) := by
   rintro x y h
@@ -133,108 +208,208 @@ termination_by w => w.length
 -- @[simp] lemma nil_inj : (nil x : Walk α β) = nil y ↔ x = y := by
 --   rw [nil.injEq]
 
+@[simp] lemma nil_validIn : (nil x : Walk α β).ValidIn G ↔ x ∈ G.V := by
+  simp only [ValidIn]
+
+@[simp] lemma nil_isWalkFrom : G.IsWalkFrom S T (nil x) ↔ x ∈ G.V ∧ x ∈ S ∧ x ∈ T := by
+  refine ⟨fun ⟨h, hS, hT⟩ ↦ ?_, fun ⟨hV, hS, hT⟩ ↦ ⟨?_, ?_, ?_⟩⟩ <;> simp_all only [and_self,
+  nil_validIn, nil_first, nil_last]
+
+@[simp] lemma nil_isTrail : G.IsTrail (nil x) ↔ x ∈ G.V := by
+  refine ⟨fun ⟨H1, H2⟩ ↦ ?_, fun h ↦ ⟨?_, ?_⟩⟩ <;> simp_all only [nil_validIn,
+    nil_edge, nodup_nil]
+
+@[simp] lemma nil_isPath : G.IsPath (nil x) ↔ x ∈ G.V := by
+  refine ⟨fun ⟨H1, H2⟩ ↦ ?_, fun h ↦ ⟨?_, ?_⟩⟩ <;> simp_all only [nil_vx,
+    nodup_cons, not_mem_nil, not_false_eq_true, nodup_nil, and_self, nil_validIn]
+
+@[simp] lemma nil_isTrailFrom : G.IsTrailFrom S T (nil x) ↔ x ∈ G.V ∧ x ∈ S ∧ x ∈ T := by
+  constructor
+  · rintro ⟨hT, hfirst, hlast⟩
+    simp_all only [nil_isTrail, nil_first, nil_last, and_self]
+  · rintro ⟨hV, hS, hT⟩
+    refine ⟨?_, ?_, ?_⟩ <;> simp_all only [nil_isTrail, IsTrail.validIn_simp, nil_edge,
+      nodup_nil, isTrail_simp, nil_first, nil_last]
+
+@[simp] lemma nil_isPathFrom : G.IsPathFrom S T (nil x) ↔ x ∈ G.V ∧ x ∈ S ∧ x ∈ T := by
+  constructor
+  · rintro ⟨hP, hfirst, hlast⟩
+    simp_all only [nil_isPath, nil_first, nil_last, and_self]
+  · rintro ⟨hV, hS, hT⟩
+    refine ⟨?_, ?_, ?_⟩ <;> simp_all only [nil_isPath, IsPath.validIn_simp, nil_edge,
+      nodup_nil, isPath_simp, nil_first, nil_last]
+
+/- Properties of cons -/
+
+@[simp] lemma cons_nonempty : (cons x e w).Nonempty := by simp [Nonempty]
+
+@[simp] lemma cons_first : (cons x e w).first = x := rfl
+
+@[simp] lemma cons_last : (cons x e w).last = w.last := rfl
+
+@[simp] lemma cons_vx : (cons x e w).vx = x :: w.vx := rfl
+
+@[simp] lemma mem_cons_iff : x ∈ (cons u e w) ↔ x = u ∨ x ∈ w := by simp [← mem_notation]
+
+@[simp] lemma cons_vxSet : (cons x e w).vxSet = {x} ∪ w.vxSet := by
+  simp only [vxSet, mem_cons_iff, singleton_union]
+  rfl
+
+@[simp↓] lemma cons_vxSet_subset : (cons x e w).vxSet ⊆ U ↔ x ∈ U ∧ w.vxSet ⊆ U := by
+  simp [insert_subset_iff]
+
 @[simp] lemma cons_edge : (cons x e w).edge = e :: w.edge := rfl
 
-@[simp] lemma cons_start : (cons x e w).start = x := rfl
+@[simp] lemma cons_edgeSet : (cons x e w).edgeSet = {e} ∪ w.edgeSet := by
+  simp only [edgeSet, cons_edge, mem_cons, singleton_union]
+  rfl
 
-@[simp] lemma cons_finish : (cons x e w).finish = w.finish := rfl
+@[simp] lemma cons_length : (cons x e w).length = w.length + 1 := rfl
 
-@[simp] lemma cons_ValidIn (hw : w.ValidIn G) (he : G.Inc₂ e x w.start) :
-  (cons x e w).ValidIn G := ⟨he, hw⟩
+@[simp] lemma cons_validIn : (cons x e w).ValidIn G ↔ G.Inc₂ e x w.first ∧ w.ValidIn G :=
+  ⟨id, id⟩
 
-@[simp] lemma cons_ValidIn_iff : (cons x e w).ValidIn G ↔ G.Inc₂ e x w.start ∧ w.ValidIn G :=
-  ⟨fun h => h, fun h => h⟩
-
-lemma ValidIn.of_cons (hw : (cons x e w).ValidIn G) : w.ValidIn G := by
-  rw [cons_ValidIn_iff] at hw
+@[simp]
+lemma ValidIn.cons (hw : (cons x e w).ValidIn G) : w.ValidIn G := by
+  rw [cons_validIn] at hw
   exact hw.2
 
+@[simp] lemma cons_isWalkFrom : G.IsWalkFrom S T (cons x e w) ↔
+    w.ValidIn G ∧ G.Inc₂ e x w.first ∧ x ∈ S ∧ w.last ∈ T := by
+  refine ⟨fun ⟨h, hS, hT⟩ ↦ ⟨?_, ?_, ?_, ?_⟩, fun ⟨hV, hS, hVd, hT⟩ ↦ ⟨?_, ?_, ?_⟩⟩
+  <;> simp_all only [cons_validIn, cons_first, cons_last, and_self]
+
+@[simp]
 lemma cons_vx_nodup (h : (cons x e w).vx.Nodup) : w.vx.Nodup := by
   simp only [cons_vx, nodup_cons] at h
   exact h.2
+
+@[simp] lemma cons_isTrail : G.IsTrail (cons x e w) ↔
+    G.IsTrail w ∧ G.Inc₂ e x w.first ∧ e ∉ w.edge := by
+  refine ⟨fun ⟨H1, H2⟩ ↦ ⟨⟨?_, ?_⟩, ?_, ?_⟩, fun ⟨hT, h₂, hnin⟩ ↦ ⟨?_, ?_⟩⟩
+  · rw [cons_validIn] at H1
+    exact H1.2
+  · simp only [cons_edge, nodup_cons] at H2
+    exact H2.2
+  · rw [cons_validIn] at H1
+    exact H1.1
+  · simp only [cons_edge, nodup_cons] at H2
+    exact H2.1
+  · simp [h₂, hT]
+  · simp [hT.edge_nodup, hnin]
+
+@[simp] lemma cons_isPath : G.IsPath (cons x e w) ↔ G.IsPath w ∧ G.Inc₂ e x w.first ∧ x ∉ w := by
+  constructor
+  · refine fun ⟨hVd, hnodup⟩ ↦ ⟨?_, ?_, ?_⟩ <;> simp_all only [cons_validIn, cons_vx,
+    nodup_cons, mem_notation, not_false_eq_true, isPath_simp]
+  · refine fun ⟨hP, h₂, hnin⟩ ↦ ⟨?_, ?_⟩ <;> simp_all only [not_false_eq_true,
+    and_self, cons_vx, nodup_cons, mem_notation, true_and, hP.validIn, hP.nodup, cons_validIn]
+
+@[simp]
+lemma cons_isTrailFrom : G.IsTrailFrom S T (cons x e w) ↔
+    G.IsTrail w ∧ G.Inc₂ e x w.first ∧ e ∉ w.edge ∧ x ∈ S ∧ w.last ∈ T := by
+  constructor
+  · refine fun ⟨⟨hVd, hnodup⟩, hfirst, hlast⟩ ↦ ⟨?_, ?_, ?_, ?_, ?_⟩ <;>
+      simp_all only [cons_validIn,
+    cons_edge, nodup_cons, cons_first, cons_last, isTrail_simp, not_false_eq_true]
+  · refine fun ⟨hV, hS, hVd, hT⟩ ↦ ⟨⟨?_, ?_⟩, ?_, ?_⟩ <;> simp_all only [IsTrail.validIn_simp,
+    not_false_eq_true, and_self, cons_edge, nodup_cons, true_and, cons_isTrail, cons_first,
+    cons_last, hV.edge_nodup]
+
+@[simp]
+lemma cons_isPathFrom : G.IsPathFrom S T (cons x e w) ↔
+    G.IsPath w ∧ G.Inc₂ e x w.first ∧ x ∉ w ∧ x ∈ S ∧ w.last ∈ T := by
+  refine ⟨fun ⟨⟨hVd, hnodup⟩, hfirst, hlast⟩ ↦ ⟨?_, ?_, ?_, ?_, ?_⟩,
+    fun ⟨hV, hS, hVd, hT⟩ ↦ ⟨⟨?_, ?_⟩, ?_, ?_⟩⟩
+  <;> simp_all only [not_false_eq_true, and_self, cons_edge, nodup_cons, cons_validIn, cons_first,
+  cons_last, mem_notation, cons_vx, isPath_simp, cons_isPath, true_and, IsPath.validIn]
+  exact hV.nodup
+
+end Walk
+open Walk
+
+@[simp]
+lemma IsTrail.cons (h : G.IsTrail (cons x e w)) : G.IsTrail w := by
+  rw [cons_isTrail] at h
+  exact h.1
+
+@[simp]
+lemma IsPath.cons (h : G.IsPath (cons x e w)) : G.IsPath w := by
+  rw [cons_isPath] at h
+  exact h.1
+
+namespace Walk
+
+/- Properties between the basic properties of a walk -/
 
 lemma vx_ne_nil : w.vx ≠ [] := by
   match w with
   | nil x => simp
   | cons x e w => simp
 
-@[simp]
-lemma mem_vx_nil_iff : x ∈ (nil u : Walk α β) ↔ x = u := by
-  simp only [mem_iff, nil_vx, mem_cons, not_mem_nil, or_false]
+@[simp] lemma mem_vxSet_iff : x ∈ w.vxSet ↔ x ∈ w := by simp [vxSet]
 
-@[simp]
-lemma mem_vx_cons_iff : x ∈ (cons u e w) ↔ x = u ∨ x ∈ w := by
-  simp only [mem_iff, cons_vx, mem_cons]
+@[simp] lemma mem_edgeSet_iff : e ∈ w.edgeSet ↔ e ∈ w.edge := by simp [edgeSet]
 
-@[simp]
-lemma mem_edge_nil_iff : e ∈ (nil u : Walk α β).edge ↔ False := by
-  simp only [nil_edge, mem_nil_iff]
-
-@[simp]
-lemma mem_edge_cons_iff : e ∈ (cons u e' w).edge ↔ e = e' ∨ e ∈ w.edge := by
-  simp only [cons_edge, mem_cons]
-
-@[simp]
-lemma start_vx_mem : w.start ∈ w.vx := by
+@[simp] lemma first_mem : w.first ∈ w := by
   match w with
-  | nil x => simp only [nil_vx, nil_start, mem_cons, not_mem_nil, or_false]
-  | cons x e w => simp only [cons_vx, cons_start, mem_cons, true_or]
+  | nil x => simp
+  | cons x e w => simp
 
-lemma start_eq_vx_head {w : Walk α β} : w.start = w.vx.head vx_ne_nil := by
+@[simp] lemma first_mem_vxSet : w.first ∈ w.vxSet := by simp
+
+lemma first_eq_vx_head : w.first = w.vx.head vx_ne_nil := by
   match w with
   | nil x => rfl
   | cons x e w => rfl
 
 @[simp]
-lemma finish_vx_mem {w : Walk α β} : w.finish ∈ w.vx := by
+lemma last_mem {w : Walk α β} : w.last ∈ w := by
   match w with
   | nil x => simp
-  | cons x e w =>
-    simp only [cons_vx, cons_finish, mem_cons]
-    right
-    exact finish_vx_mem
+  | cons x e w => simp [last_mem]
 
-lemma finish_eq_vx_getLast {w : Walk α β} : w.finish = w.vx.getLast vx_ne_nil := by
+@[simp]
+lemma last_mem_vxSet : w.last ∈ w.vxSet := by simp
+
+lemma last_eq_vx_getLast {w : Walk α β} : w.last = w.vx.getLast vx_ne_nil := by
   match w with
   | nil x => rfl
   | cons x e w =>
-    simp only [cons_finish, cons_vx, ne_eq, vx_ne_nil, not_false_eq_true, getLast_cons]
-    apply finish_eq_vx_getLast
+    simp only [cons_last, cons_vx, ne_eq, vx_ne_nil, not_false_eq_true, getLast_cons]
+    apply last_eq_vx_getLast
 
-lemma ValidIn.mem_of_mem_vx {w : Walk α β} (h : w.ValidIn G) (hmem : x ∈ w.vx) :
-    x ∈ G.V := by
+lemma ValidIn.vx_mem_of_mem {w : Walk α β} (h : w.ValidIn G) (hmem : x ∈ w) : x ∈ G.V := by
   match w with
-  | nil y =>
-    simp only [nil_vx, mem_cons, not_mem_nil, or_false] at hmem
-    subst x
-    exact h
-  | cons y e w =>
+  | .nil y =>
+    rw [mem_nil_iff] at hmem
+    exact mem_of_eq_of_mem hmem h
+  | .cons y e w =>
     obtain ⟨hbtw, hVd⟩ := h
-    obtain rfl | h : x = y ∨ x ∈ w.vx := by simpa using hmem
+    obtain rfl | h : x = y ∨ x ∈ w := by simpa using hmem
     · exact hbtw.vx_mem_left
-    · exact hVd.mem_of_mem_vx h
+    · exact hVd.vx_mem_of_mem h
 
-lemma ValidIn.mem_of_mem_edge {w : Walk α β} (h : w.ValidIn G) (hmem : e ∈ w.edge) :
-    e ∈ G.E := by
+lemma ValidIn.vxSet_subset (hVd : w.ValidIn G) : w.vxSet ⊆ G.V := fun _ ↦ hVd.vx_mem_of_mem
+
+lemma ValidIn.edge_mem_of_mem {w : Walk α β} (h : w.ValidIn G) (hmem : e ∈ w.edge) : e ∈ G.E := by
   match w with
-  | nil x => simp at hmem
-  | cons x e' w =>
+  | .nil x => simp at hmem
+  | .cons x e' w =>
     obtain ⟨hbtw, hVd⟩ := h
     obtain rfl | h : e = e' ∨ e ∈ w.edge := by simpa using hmem
     · exact hbtw.edge_mem
-    · exact hVd.mem_of_mem_edge h
+    · exact hVd.edge_mem_of_mem h
 
+lemma ValidIn.edgeSet_subset (h : w.ValidIn G) : w.edgeSet ⊆ G.E := fun _ ↦ h.edge_mem_of_mem
 
-lemma Nonempty.exists_cons : w.Nonempty → ∃ x e w', w = cons x e w' := by
-  induction w with
-  | nil x => simp only [Nonempty, reduceCtorEq, exists_false, imp_self]
-  | cons x e w ih => simp only [cons.injEq, exists_and_left, exists_eq', and_true, implies_true]
+/- Properties of Nonempty -/
 
-lemma Nonempty.iff_exists_cons : w.Nonempty ↔ ∃ x e w', w = cons x e w' := by
-  constructor
-  · apply Nonempty.exists_cons
-  · rintro ⟨x, e, w', rfl⟩
-    simp only [Nonempty, cons.injEq, exists_and_left, exists_eq', and_true, implies_true]
+lemma Nonempty.exists_cons (hw : w.Nonempty) : ∃ x e w', w = cons x e w' := by
+  induction w with simp_all
+
+lemma nonempty_iff_exists_cons : w.Nonempty ↔ ∃ x e w', w = cons x e w' := by
+  induction w with simp
 
 @[simp]
 lemma Nonempty.not_nil : ¬ (nil x : Walk α β).Nonempty := by
@@ -251,200 +426,185 @@ lemma Nonempty.not_iff : ¬ w.Nonempty ↔ ∃ x, w = nil x := by
   | cons x e w => simp only [Nonempty, not_true_eq_false, reduceCtorEq, exists_false]
 
 @[simp]
-lemma length_pos_iff : 0 < w.length ↔ w.Nonempty := by
+lemma Nonempty.iff_length_pos : 0 < w.length ↔ w.Nonempty := by
   induction w with simp
 
-lemma start_eq_finish_of_not_nonempty (h : ¬ w.Nonempty) : w.start = w.finish := by
+lemma first_eq_last_of_not_nonempty (h : ¬ w.Nonempty) : w.first = w.last := by
   match w with
-  | nil x => simp only [nil_start, nil_finish]
+  | nil x => simp only [nil_first, nil_last]
   | cons x e w => simp only [Nonempty.cons_true, not_true_eq_false] at h
 
 @[simp]
-lemma start_eq_finish_iff (hnodup : w.vx.Nodup) : w.start = w.finish ↔ ¬ w.Nonempty := by
+lemma first_eq_last_iff (hnodup : w.vx.Nodup) : w.first = w.last ↔ ¬ w.Nonempty := by
   match w with
-  | .nil x => simp only [nil_start, nil_finish, Nonempty.not_nil, not_false_eq_true]
+  | .nil x => simp only [nil_first, nil_last, Nonempty.not_nil, not_false_eq_true]
   | .cons x e w =>
-    simp only [cons_vx, nodup_cons, cons_start, cons_finish, Nonempty.cons_true, not_true_eq_false,
+    simp only [cons_vx, nodup_cons, cons_first, cons_last, Nonempty.cons_true, not_true_eq_false,
       iff_false, ne_eq] at hnodup ⊢
-    exact fun h => hnodup.1 (h ▸ finish_vx_mem)
+    exact fun h => hnodup.1 (h ▸ last_mem)
 
 @[simp]
-lemma start_ne_finish_iff (hnodup : w.vx.Nodup) : w.start ≠ w.finish ↔ w.Nonempty :=
-  (start_eq_finish_iff hnodup).not_left
+lemma first_ne_last_iff (hnodup : w.vx.Nodup) : w.first ≠ w.last ↔ w.Nonempty :=
+  (first_eq_last_iff hnodup).not_left
 
-/- Properties of append operation -/
-@[simp]
-lemma append_notation : append w₁ w₂ = w₁ ++ w₂ := rfl
+end Walk
+open Walk
 
-@[simp]
-lemma nil_append : nil x ++ w₂ = w₂ := by
-  simp only [← append_notation, append]
+lemma IsPath.not_isCycle (hP : G.IsPath w) (hnonempty : w.Nonempty) : ¬ G.IsCycle w := by
+  suffices heq : w.first ≠ w.last by
+    rintro ⟨hVd, hnodup, hclosed⟩
+    exact heq hclosed
+  rwa [first_ne_last_iff hP.nodup]
 
-@[simp]
-lemma cons_append : cons x e w₁ ++ w₂ = cons x e (w₁ ++ w₂) := by
-  simp only [← append_notation, append]
+def Inc₂.walk (_h : G.Inc₂ e u v) : Walk α β := cons u e (nil v)
 
-@[simp]
-lemma append_vx : (w₁ ++ w₂).vx = w₁.vx.dropLast ++ w₂.vx := by
-  induction w₁ with
-  | nil x => simp
-  | cons x e w ih =>
-    simp only [append_notation, append, cons_vx]
-    rw [List.dropLast_cons_of_ne_nil vx_ne_nil, List.cons_append]
-    simpa
+namespace Inc₂
 
-lemma append_vx' {w₁ w₂ : Walk α β} (heq : w₁.finish = w₂.start) :
-    (w₁ ++ w₂).vx = w₁.vx ++ w₂.vx.tail := by
-  match w₁ with
-  | .nil x =>
-    simp_all only [nil_finish, append_vx, nil_vx, dropLast_single, nil_append, cons_append]
-    rw [start_eq_vx_head]
-    exact (head_cons_tail w₂.vx vx_ne_nil).symm
-  | .cons x e w =>
-    simp only [cons_finish, cons_append, cons_vx, List.cons_append, List.cons.injEq,
-      true_and] at heq ⊢
-    exact append_vx' heq
+@[simp] lemma walk_first (h : G.Inc₂ e u v): h.walk.first = u := rfl
 
-@[simp]
-lemma append_edge {w₁ w₂ : Walk α β} : (w₁ ++ w₂).edge = w₁.edge ++ w₂.edge := by
-  induction w₁ with
-  | nil x => simp only [nil_append, nil_edge, List.nil_append]
-  | cons x e w ih => simp only [cons_append, cons_edge, ih, List.cons_append]
+@[simp] lemma walk_last (h : G.Inc₂ e u v): h.walk.last = v := rfl
 
-@[simp]
-lemma append_length : (w₁ ++ w₂).length = w₁.length + w₂.length := by
-  induction w₁ with
-  | nil x => simp
-  | cons x e w ih => simp [ih, Nat.add_right_comm]
+@[simp] lemma walk_vx (h : G.Inc₂ e u v): h.walk.vx = [u, v] := rfl
 
-@[simp]
-lemma append_nil (h : w.finish = x) : w ++ (nil x) = w := by
-  induction w with
-  | nil u => aesop
-  | cons u e W ih =>
-    rw [cons_finish] at h
-    rw [cons_append, ih h]
+@[simp] lemma mem_walk_iff (h : G.Inc₂ e u v) (x : α) : x ∈ h.walk ↔ x = u ∨ x = v := by
+  simp [walk]
 
-@[simp]
-lemma append_start_of_eq (h : w₁.finish = w₂.start):
-  (w₁ ++ w₂).start = w₁.start := by
-  induction w₁ with
-  | nil x => simp only [nil_append, ← h, nil_finish, nil_start]
-  | cons x e w ih => simp only [cons_append, cons_start]
-
-@[simp]
-lemma append_start_of_nonempty (h : w₁.Nonempty) :
-  (w₁ ++ w₂).start = w₁.start := by
-  induction w₁ with
-  | nil x => simp only [Nonempty.not_nil] at h
-  | cons x e w ih => simp only [cons_append, cons_start]
-
-@[simp]
-lemma append_finish :
-  (w₁ ++ w₂).finish = w₂.finish := by
-  induction w₁ with
-  | nil x => simp only [nil_append]
-  | cons x e w ih => simp only [cons_append, cons_finish, ih]
-
-lemma append_assoc (w1 w2 w3 : Walk α β) : (w1 ++ w2) ++ w3 = w1 ++ (w2 ++ w3) := by
-  induction w1 with
-  | nil x => simp only [nil_append]
-  | cons x e w ih => simp only [cons_append, ih]
-
-lemma append_right_injective : Injective (w ++ ·) := by
-  rintro w₁ w₂ h
-  induction w with
-  | nil x => simpa only [nil_append] using h
-  | cons x e w ih =>
-    simp only [cons_append, cons.injEq, true_and] at h
-    exact ih h
-
-@[simp]
-lemma append_right_inj : w ++ w₁ = w ++ w₂ ↔ w₁ = w₂ := by
-  constructor
-  · apply append_right_injective
-  · rintro rfl
-    rfl
-
-@[simp]
-lemma append_right_eq_self : w ++ w₁ = w ↔ w₁ = nil w.finish := by
-  induction w with
-  | nil x => simp only [nil_append, nil_finish]
-  | cons x e w ih => simpa only [cons_append, cons.injEq, true_and, cons_finish]
-
-@[simp]
-lemma append_left_eq_self : w₁ ++ w = w ↔ ¬ w₁.Nonempty := by
-  refine ⟨fun h ↦ by simpa [← length_pos_iff] using congr_arg length h, fun h ↦ ?_⟩
-  obtain ⟨x, rfl⟩ := by simpa using h
+@[simp] lemma walk_vxSet (h : G.Inc₂ e u v): h.walk.vxSet = {u, v} := by
+  simp only [vxSet, mem_walk_iff]
   rfl
 
+@[simp] lemma walk_edge (h : G.Inc₂ e u v): h.walk.edge = [e] := rfl
+
+@[simp] lemma walk_edgeSet (h : G.Inc₂ e u v): h.walk.edgeSet = {e} := by simp [edgeSet]
+
+@[simp] lemma walk_length (h : G.Inc₂ e u v): h.walk.length = 1 := rfl
+
 @[simp]
-lemma append_eq_nil_iff : w₁ ++ w₂ = nil x ↔ (∃ y, w₁ = nil y) ∧ w₂ = nil x := by
-  induction w₁ with
-  | nil y => simp only [nil_append, nil.injEq, exists_eq', true_and]
-  | cons y e w ih => simp only [cons_append, reduceCtorEq, exists_false, false_and]
+lemma walk_validIn (h : G.Inc₂ e u v) : h.walk.ValidIn G := by
+  simp [walk, h, h.vx_mem_right]
 
-lemma append_ValidIn (h : w₁.finish = w₂.start) (h₁ : w₁.ValidIn G) (h₂ : w₂.ValidIn G) :
-  (w₁ ++ w₂).ValidIn G := by
-  induction w₁ with
-  | nil x => simpa
-  | cons x e w₁ ih =>
-    simp only [cons_finish] at h
-    refine ⟨?_, by simp [ih h h₁.2]⟩
-    convert h₁.1 using 1
-    exact append_start_of_eq h
+lemma walk_isPath (h : G.Inc₂ e u v) (hne : u ≠ v) : G.IsPath h.walk :=
+  ⟨h.walk_validIn, by simp [hne]⟩
 
-lemma ValidIn.append_left_ValidIn (h : w₁.finish = w₂.start) (hw₁ : w₁.Nonempty)
-    (hVd : (w₁ ++ w₂).ValidIn G) : w₁.ValidIn G := by
-  induction w₁ with
-  | nil x => simp only [Nonempty.not_nil] at hw₁
-  | cons x e w ih =>
-    simp only [cons_append, cons_ValidIn_iff] at hVd
-    by_cases hNonempty : w.Nonempty
-    · refine ⟨?_, ih h hNonempty hVd.2⟩
-      convert hVd.1 using 1
-      simp only [hNonempty, append_start_of_nonempty]
-    · simp only [Nonempty.not_iff] at hNonempty
-      obtain ⟨y, rfl⟩ := hNonempty
-      simp only [cons_finish, nil_finish, nil_append, cons_ValidIn_iff, nil_start,
-        nil_ValidIn_iff] at h hVd ⊢
-      subst y
-      refine ⟨hVd.1, hVd.2.mem_of_mem_vx start_vx_mem⟩
+lemma ValidIn.mem_of_mem_edge_of_inc (hVd : w.ValidIn G) (he : e ∈ w.edge) (h : G.Inc e u) :
+    u ∈ w := by
+  induction w with
+  | nil x => simp at he
+  | cons x e' w ih =>
+  simp only [mem_cons_iff, or_iff_not_imp_left]
+  simp only [cons_validIn] at hVd
+  intro hux
+  obtain rfl | h' : e = e' ∨ _ := by simpa using he
+  · simp [h.eq_of_inc₂_of_ne_left hVd.1 hux]
+  exact ih hVd.2 h'
 
-lemma ValidIn.append_right_ValidIn (hVd : (w₁ ++ w₂).ValidIn G) : w₂.ValidIn G := by
-  induction w₁ with
-  | nil x => simpa only [nil_append] using hVd
-  | cons x e w ih =>
-    simp only [cons_append, cons_ValidIn_iff] at hVd
-    exact ih hVd.2
-
-lemma ValidIn.finish_eq_start (hw₁ : w₁.Nonempty) (hVd₁ : w₁.ValidIn G) (hVd : (w₁ ++ w₂).ValidIn G) :
-  w₁.finish = w₂.start := by
+end Inc₂
 
 
-  match w₁ with
-  | nil x => simp at hw₁
-  | cons x e w₁ =>
-  induction w₁ with
-  | nil u =>
-  simp_all only [Nonempty.cons_true, cons_ValidIn_iff, nil_start, nil_ValidIn_iff, cons_append,
-    nil_append, cons_finish, nil_finish]
-  exact hVd₁.1.eq_of_inc₂ hVd.1
-  | cons u f w₁ ih =>
-  simp_all only [Nonempty.cons_true, cons_ValidIn_iff, cons_append, cons_finish, and_imp,
-    forall_const, cons_start, true_and, implies_true]
 
-  rw [append_start_of_nonempty] at hVd
+-- /-- Given a graph adjacency, we can create a walk of length 1 -/
+-- lemma Adj.exist_walk (h : G.Adj u v) : ∃ (W : Walk α β), W.ValidIn G ∧ W.length = 1 ∧
+-- W.first = u ∧
+--     W.last = v := by
+--   obtain ⟨e, he⟩ := h
+--   use he.walk, he.walk_validIn
+--   simp only [Inc₂.walk_length, Inc₂.walk_first, Inc₂.walk_last, and_self]
+
+-- /-- Given a reflexive adjacency, we can create a walk of length at most 1 -/
+-- -- lemma reflAdj.exist_walk (h : G.reflAdj u v) : ∃ (W : Walk α β), W.ValidIn G ∧ W.length ≤ 1 ∧
+-- --     W.first = u ∧ W.last = v := by
+-- --   obtain hadj | ⟨rfl, hx⟩ := h
+-- --   · obtain ⟨W, hW, hlength, hfirst, hlast⟩ := hadj.exist_walk
+-- --     use W, hW
+-- --     simp only [hlength, le_refl, hfirst, hlast, and_self]
+-- --   · use nil u
+-- --     constructor
+-- --     · simp [hx]
+-- --     · simp
+
+-- namespace Walk.ValidIn
+
+-- lemma connected (h : w.ValidIn G) : G.Connected w.first w.last := by
+--   induction w with
+--   | nil x => simpa only [nil_first, nil_last, Connected.refl_iff]
+--   | cons x e w ih =>
+--     obtain ⟨H1, H2⟩ := h
+--     simp only [cons_first, cons_last]
+--     exact H1.connected.trans (ih H2)
+
+-- lemma connected_last_of_mem (h : w.ValidIn G) (hx : u ∈ w) : G.Connected u w.last := by
+--   induction w generalizing u with
+--   | nil x =>
+--     rw [mem_nil_iff] at hx
+--     subst u
+--     simp only [nil_last, Connected.refl_iff]
+--     exact h
+--   | cons x e w ih =>
+--     rw [mem_cons_iff] at hx
+--     obtain rfl | hx := hx
+--     · exact Connected.trans h.1.connected (ih h.2 (first_mem))
+--     · exact ih h.2 hx
+
+-- lemma connected_of_mem (h : w.ValidIn G) (hx : x ∈ w) (hy : y ∈ w) :
+--     G.Connected x y := by
+--   have hx' := connected_last_of_mem h hx
+--   have hy' := connected_last_of_mem h hy
+--   exact Connected.trans hx' hy'.symm
+
+-- lemma connected_first_of_mem (h : w.ValidIn G) (hx : x ∈ w) : G.Connected w.first x :=
+--   h.connected_of_mem first_mem hx
+
+-- lemma eq_nil_of_mem_isolated {w : Walk α β} {x : α} (hisol : G.Isolated x) (hmem : x ∈ w)
+--     (h : w.ValidIn G) : w = nil x := by
+--   match w with
+--   | .nil y => simp_all only [mem_nil_iff, nil_validIn]
+--   | .cons y e w =>
+--     exfalso
+--     obtain ⟨hbtw, hVd⟩ := h
+--     rw [mem_cons_iff] at hmem
+--     obtain rfl | h := hmem
+--     · exact hisol e hbtw.inc_left
+--     · have := eq_nil_of_mem_isolated hisol h hVd
+--       subst w
+--       rw [nil_first] at hbtw
+--       exact hisol e hbtw.inc_right
+
+-- end Walk.ValidIn
+
+-- namespace IsWalkFrom
+
+-- lemma setConnected (hWF : G.IsWalkFrom S T w) : G.SetConnected S T := by
+--   obtain ⟨hVd, hfirst, hlast⟩ := hWF
+--   use w.first, hfirst, w.last, hlast, hVd.connected
+
+-- lemma left_subset (hWF : G.IsWalkFrom S T w) (hsubset : S ∩ G.V ⊆ S') : G.IsWalkFrom S' T w where
+--   validIn := hWF.validIn
+--   first_mem := hsubset ⟨hWF.first_mem, hWF.validIn.vx_mem_of_mem Walk.first_mem⟩
+--   last_mem := hWF.last_mem
+
+-- lemma left_subset' (hWF : G.IsWalkFrom S T w) (hsubset : S ⊆ S') : G.IsWalkFrom S' T w where
+--   validIn := hWF.validIn
+--   first_mem := hsubset hWF.first_mem
+--   last_mem := hWF.last_mem
+
+-- lemma right_subset (hWF : G.IsWalkFrom S T w) (hsubset : T ∩ G.V ⊆ T') :
+    -- G.IsWalkFrom S T' w where
+--   validIn := hWF.validIn
+--   first_mem := hWF.first_mem
+--   last_mem := hsubset ⟨hWF.last_mem, hWF.validIn.vx_mem_of_mem Walk.last_mem⟩
+
+-- lemma right_subset' (hWF : G.IsWalkFrom S T w) (hsubset : T ⊆ T') : G.IsWalkFrom S T' w where
+--   validIn := hWF.validIn
+--   first_mem := hWF.first_mem
+--   last_mem := hsubset hWF.last_mem
+
+-- lemma left_right_subset (hWF : G.IsWalkFrom S T w) (hS : S ∩ G.V ⊆ S') (hT : T ∩ G.V ⊆ T') :
+--     G.IsWalkFrom S' T' w := hWF.left_subset hS |>.right_subset hT
+
+-- lemma left_right_subset' (hWF : G.IsWalkFrom S T w) (hS : S ⊆ S') (hT : T ⊆ T') :
+--     G.IsWalkFrom S' T' w := hWF.left_subset' hS |>.right_subset' hT
 
 
-  -- simp only [cons_append, cons_ValidIn_iff] at hVd
-  -- rw [append_start_of_nonempty] at hVd
+-- end IsWalkFrom
 
-    -- simp_all only [Nonempty.cons_true, cons_append, cons_ValidIn_iff, cons_finish, forall_const]
-    -- by_cases hNonempty : w.Nonempty
-    -- · simp_all only [forall_const, append_start_of_eq, true_and]
-    -- · simp only [Nonempty.not_iff] at hNonempty
-    --   obtain ⟨y, rfl⟩ := hNonempty
-    --   simp_all only [Nonempty.not_nil, nil_finish, IsEmpty.forall_iff, nil_start, nil_ValidIn_iff,
-    --     nil_append]
-    --   exact hVd₁.1.eq_of_Inc₂ hVd.1
+end Graph
