Matroid/ForMathlib/Graph/Connected.lean
@@ -1,0 +1,395 @@
+import Matroid.ForMathlib.Graph.Walk
+import Matroid.ForMathlib.Graph.Subgraph
+
+open Set Function List Nat
+
+variable {α β : Type*} {G H : Graph α β} {u v x y z : α} {e e' f g : β} {S S' T T' U V : Set α}
+  {F F' R R': Set β}
+
+namespace Graph
+
+
+/-- Connectedness of vertices-/
+def VxConnected (G : Graph α β) : α → α → Prop :=
+    Relation.TransGen (fun x y ↦ G.Adj x y ∨ (x = y ∧ x ∈ G.V))
+
+lemma VxConnected.refl (h : v ∈ G.V) : G.VxConnected v v := by
+  rw [VxConnected, Relation.transGen_iff]
+  simp [h]
+
+lemma VxConnected.trans (hxy : G.VxConnected x y) (hyz : G.VxConnected y z) : G.VxConnected x z :=
+  Relation.TransGen.trans hxy hyz
+
+lemma VxConnected.symm (hxy : G.VxConnected x y) : G.VxConnected y x := by
+  rw [VxConnected, Relation.transGen_swap]
+  rw [VxConnected] at hxy
+  convert hxy using 4 with x y
+  · rw [adj_comm]
+  aesop
+
+lemma VxConnected.mem_left (hxy : G.VxConnected x y) : x ∈ G.V := by
+  induction hxy with
+  | @single a h =>
+    obtain h | h := h
+    · exact h.mem_left
+    exact h.2
+  | tail _ _ h => exact h
+
+lemma VxConnected.mem_right (hxy : G.VxConnected x y) : y ∈ G.V :=
+  hxy.symm.mem_left
+
+@[simp]
+lemma vxConnected_self : G.VxConnected x x ↔ x ∈ G.V :=
+  ⟨VxConnected.mem_left, VxConnected.refl⟩
+
+
+
+lemma Adj.vxConnected (h : G.Adj x y) : G.VxConnected x y := by
+  rw [VxConnected, Relation.transGen_iff]
+  simp [h]
+
+lemma Inc₂.vxConnected (h : G.Inc₂ e x y) : G.VxConnected x y :=
+  h.adj.vxConnected
+
+lemma Walk.ValidIn.vxConnected {w : Walk α β} (hw : w.ValidIn G) :
+    G.VxConnected w.first w.last := by
+  induction w with
+  | nil u =>
+  apply VxConnected.refl
+  simpa using hw
+  | cons u e W ih =>
+  simp only [cons_first, cons_last]
+  simp only [cons_validIn] at hw
+  exact hw.1.vxConnected.trans <| ih hw.2
+
+lemma VxConnected.exists_walk_validIn (h : G.VxConnected x y) :
+    ∃ (w : Walk α β), w.ValidIn G ∧ w.first = x ∧ w.last = y := by
+  rw [VxConnected] at h
+  induction h using Relation.TransGen.head_induction_on with
+  | @base a h =>
+    obtain ⟨e, he⟩ | ⟨rfl, h⟩ := h
+    · exact ⟨he.walk, by simp⟩
+    exact ⟨Walk.nil a, by simp [h]⟩
+  | @ih u v h₁ h₂ h₃ =>
+  obtain ⟨w, hw, rfl, rfl⟩ := h₃
+  obtain ⟨e, he⟩ | ⟨rfl, h⟩ := h₁
+  · exact ⟨Walk.cons u e w, by simp [he, hw]⟩
+  exact ⟨w, hw, rfl, rfl⟩
+
+lemma vxConnected_iff_exists_walk :
+    G.VxConnected x y ↔ ∃ (w : Walk α β), w.ValidIn G ∧ w.first = x ∧ w.last = y := by
+  refine ⟨VxConnected.exists_walk_validIn, ?_⟩
+  rintro ⟨w, hw, rfl, rfl⟩
+  exact hw.vxConnected
+
+@[mk_iff]
+structure Connected (G : Graph α β) : Prop where
+  nonempty : G.V.Nonempty
+  forall_vxConnected : ∀ ⦃x y⦄, x ∈ G.V → y ∈ G.V → G.VxConnected x y
+
+lemma exists_of_not_connected (h : ¬ G.Connected) (hne : G.V.Nonempty) :
+    ∃ X ⊂ G.V, X.Nonempty ∧ ∀ ⦃u v⦄, u ∈ X → G.Adj u v → v ∈ X := by
+  obtain ⟨x, hx⟩ := hne
+  refine ⟨{y | G.VxConnected x y}, ?_, ⟨x, by simpa⟩, fun u v (h : G.VxConnected x u) huv ↦ ?_⟩
+  · refine subset_of
+
+
+-- structure VxSeparation (G : Graph α β) (k : ℕ) where
+--   left : Set α
+--   right : Set α
+--   union_eq : left ∪ right = G.V
+--   disjoint : Disjoint left right
+
+
+-- lemma exists_partition_of_not_connected {G : Graph α β} (h : ¬ G.Connected) :
+--     ∃ X Y, X.Nonempty ∧ Y.Nonempty ∧
+
+
+
+-- section Connected
+
+-- @[simp]
+-- def reflAdj (G : Graph α β) (x y : α) :=
+--   G.Adj x y ∨ x = y ∧ x ∈ G.V
+
+-- lemma reflAdj.of_vxMem (h : x ∈ G.V) : G.reflAdj x x := by
+--   simp only [reflAdj, h, and_self, or_true]
+
+-- @[simp]
+-- lemma reflAdj.refl (h : x ∈ G.V) : G.reflAdj x x := reflAdj.of_vxMem h
+
+-- lemma reflAdj.symm (h : G.reflAdj x y) : G.reflAdj y x := by
+--   apply h.imp
+--   · exact fun h ↦ h.symm
+--   · rintro ⟨rfl, hx⟩
+--     exact ⟨rfl, hx⟩
+
+-- lemma reflAdj.comm : G.reflAdj x y ↔ G.reflAdj y x := by
+--   refine ⟨reflAdj.symm, reflAdj.symm⟩
+
+-- lemma Inc.reflAdj_of_inc (hx : G.Inc e x) (hy : G.Inc e y) : G.reflAdj x y := by
+--   by_cases hxy : x = y
+--   · subst y
+--     right
+--     exact ⟨rfl, hx.vx_mem⟩
+--   · left
+--     use e
+--     rw [inc₂_iff_inc_and_loop]
+--     use hx, hy, fun h ↦ (hxy h).elim
+
+-- @[simp]
+-- lemma reflAdj.mem_left (h : G.reflAdj x y) : x ∈ G.V := by
+--   apply h.elim
+--   · exact fun a ↦ a.mem_left
+--   · tauto
+
+-- @[simp]
+-- lemma reflAdj.mem_right (h : G.reflAdj x y) : y ∈ G.V := by
+--   rw [reflAdj.comm] at h
+--   exact h.mem_left
+
+-- @[simp]
+-- lemma Inc₂.reflAdj (h : G.Inc₂ e x y) : G.reflAdj x y := by
+--   left
+--   use e
+
+-- @[simp]
+-- lemma Adj.reflAdj (h : G.Adj x y) : G.reflAdj x y := by
+--   left
+--   exact h
+
+-- lemma reflAdj.Adj_of_ne (h : G.reflAdj x y) (hne : x ≠ y) : G.Adj x y := by
+--   obtain ⟨e, h⟩ | ⟨rfl, hx⟩ := h
+--   · use e
+--   · contradiction
+
+-- @[simp]
+-- lemma reflAdj.Adj_iff_ne (hne : x ≠ y) : G.reflAdj x y ↔ G.Adj x y :=
+--   ⟨fun h => h.Adj_of_ne hne, fun h => h.reflAdj⟩
+
+-- lemma reflAdj.le (h : G.reflAdj u v) (hle : G ≤ H) : H.reflAdj u v := by
+--   obtain hadj | ⟨rfl, hu⟩ := h
+--   · left
+--     exact hadj.le hle
+--   · right
+--     simp only [vx_subset_of_le hle hu, and_self]
+
+
+-- def Connected (G : Graph α β) := Relation.TransGen G.reflAdj
+
+-- @[simp]
+-- lemma Inc₂.connected (h : G.Inc₂ e x y) : G.Connected x y :=
+--   Relation.TransGen.single h.reflAdj
+
+-- @[simp]
+-- lemma Adj.connected (h : G.Adj x y) : G.Connected x y := Relation.TransGen.single h.reflAdj
+
+-- @[simp]
+-- lemma reflAdj.connected (h : G.reflAdj x y) : G.Connected x y := Relation.TransGen.single h
+
+-- lemma connected_self (hx : x ∈ G.V) : G.Connected x x :=
+--   Relation.TransGen.single <| reflAdj.of_vxMem hx
+
+-- lemma Inc.connected_of_inc (hx : G.Inc e x) (hy : G.Inc e y) : G.Connected x y :=
+--   reflAdj.connected (hx.reflAdj_of_inc hy)
+
+-- lemma Connected.comm : G.Connected x y ↔ G.Connected y x := by
+--   unfold Connected
+--   rw [Relation.transGen_swap]
+--   congr! 1
+--   ext
+--   exact reflAdj.comm
+
+-- @[simp]
+-- lemma Connected.refl (hx : x ∈ G.V) : G.Connected x x :=
+--   connected_self hx
+
+-- @[simp]
+-- lemma Connected.exists_connected (hx : x ∈ G.V) : ∃ y, G.Connected x y := by
+--   use x, Connected.refl hx
+
+-- lemma Connected.symm (h : G.Connected x y) : G.Connected y x := by
+--   rwa [Connected.comm]
+
+-- instance : IsSymm α (G.Connected) := ⟨fun _ _ ↦ Connected.symm⟩
+
+-- lemma Connected.trans (hxy : G.Connected x y) (hyz : G.Connected y z) :
+--     G.Connected x z := Relation.TransGen.trans hxy hyz
+
+-- instance : IsTrans α (G.Connected) := ⟨fun _ _ _ ↦ Connected.trans⟩
+
+-- @[simp]
+-- lemma Connected.mem_left (hconn : G.Connected x y) : x ∈ G.V := by
+--   simp only [Connected, Relation.TransGen.head'_iff, not_exists, not_and, not_or] at hconn
+--   obtain ⟨a, hradj, hTG⟩ := hconn
+--   exact hradj.mem_left
+
+-- @[simp]
+-- lemma Connected.mem_right (hconn : G.Connected x y) : y ∈ G.V := by
+--   rw [Connected.comm] at hconn
+--   exact hconn.mem_left
+
+-- @[simp]
+-- lemma not_connected_of_not_mem (h : x ∉ G.V) : ¬G.Connected x y := by
+--   contrapose! h
+--   exact h.mem_left
+
+-- @[simp]
+-- lemma not_connected_of_not_mem' (h : y ∉ G.V) : ¬G.Connected x y := by
+--   rw [Connected.comm]
+--   exact not_connected_of_not_mem h
+
+-- @[simp]
+-- lemma Connected.refl_iff : G.Connected x x ↔ x ∈ G.V := by
+--   refine ⟨?_, Connected.refl⟩
+--   rintro h
+--   exact h.mem_left
+
+-- lemma Connected.le (h : G.Connected u v) (hle : G ≤ H) : H.Connected u v := by
+--   induction h with
+--   | single huv => exact Relation.TransGen.single (huv.le hle)
+--   | tail huv h ih => exact Relation.TransGen.tail ih (h.le hle)
+
+-- class Conn (G : Graph α β) : Prop where
+--   all_conn : ∃ x, ∀ y ∈ G.V, G.Connected x y
+
+-- open Partition
+
+-- def ConnectedPartition (G : Graph α β) : Partition (Set α) := Partition.ofRel (G.Connected)
+
+-- def Component (G : Graph α β) (v : α) := {u | G.Connected v u}
+
+-- def ComponentSets (G : Graph α β) (V : Set α) := {Component G u | u ∈ V}
+
+-- @[simp]
+-- lemma ComponentPartition.supp : G.ConnectedPartition.supp = G.V := by
+--   simp [ConnectedPartition]
+
+-- @[simp]
+-- lemma set_spec_connected_comm : {x | G.Connected x y} = {x | G.Connected y x} := by
+--   simp_rw [Connected.comm]
+
+-- @[simp] lemma set_spec_connected_eq_componentSet : {x | G.Connected y x} = G.Component y := rfl
+
+-- @[simp]
+-- lemma Component.empty : G.Component x = ∅ ↔ x ∉ G.V := by
+--   constructor
+--   · intro h hx
+--     rw [← mem_empty_iff_false, ← h]
+--     exact Connected.refl hx
+--   · intro h
+--     ext y
+--     simp [Component, h]
+
+-- @[simp]
+-- lemma Component.eq (hx : x ∈ G.V) : G.Component x = G.Component y ↔ G.Connected x y :=
+--   (rel_iff_eqv_class_eq_left (Connected.refl hx)).symm
+
+-- @[simp]
+-- lemma Component.eq' (hy : y ∈ G.V) : G.Component x = G.Component y ↔ G.Connected x y := by
+--   rw [eq_comm, Connected.comm, eq hy]
+
+-- @[simp]
+-- lemma Component.mem_partition : G.Component x ∈ G.ConnectedPartition ↔ x ∈ G.V := by
+--   refine mem_ofRel_iff.trans ?_
+--   simp +contextual only [Connected.refl_iff, set_spec_connected_eq_componentSet, iff_def,
+--     forall_exists_index, and_imp, eq', eq]
+--   refine ⟨fun y hy hconn ↦ hconn.mem_left, fun h ↦ ?_⟩
+--   use x, h, Connected.refl h
+
+-- @[simp] lemma Component.mem : y ∈ G.Component x ↔ G.Connected x y := by rfl
+
+-- lemma Component.mem' : y ∈ G.Component x ↔ G.Connected y x := by
+--   rw [Connected.comm, Component.mem]
+
+-- -- @[simp] lemma ComponentSet.self_mem : x ∈ G.ComponentSet x ↔ x ∈ G.V := by simp
+
+-- @[simp]
+-- lemma ComponentSets.mem (hx : x ∈ G.V) :
+--     G.Component x ∈ G.ComponentSets T ↔ ∃ y ∈ T, G.Connected x y := by
+--   simp only [ComponentSets, mem_setOf_eq, hx, Component.eq']
+--   simp_rw [Connected.comm]
+
+-- lemma ComponentSets.componentSet (hx : x ∈ G.V) :
+--     G.ComponentSets (G.Component x) = {G.Component x} := by
+--   ext S
+--   simp +contextual only [mem_singleton_iff, iff_def, hx, mem, Component.mem, and_self,
+--     Connected.exists_connected, implies_true, and_true]
+--   rintro ⟨y, hy, rfl⟩
+--   simpa [hx, Connected.comm] using hy
+
+-- lemma ConnectedPartition.le (hle : G ≤ H) : G.ConnectedPartition ≤ H.ConnectedPartition := by
+--   simpa [ConnectedPartition] using fun u v ↦ (Connected.le · hle)
+
+-- @[simp]
+-- lemma ConnectedPartition.Rel : G.ConnectedPartition.Rel = G.Connected := by
+--   unfold ConnectedPartition
+--   rw [rel_ofRel_eq]
+
+-- def SetConnected (G : Graph α β) (S T : Set α) : Prop := ∃ s ∈ S, ∃ t ∈ T, G.Connected s t
+
+-- namespace SetConnected
+-- variable {G : Graph α β} {S S' T T' U V : Set α}
+
+-- lemma refl (h : ∃ x ∈ S, x ∈ G.V) : G.SetConnected S S := by
+--   obtain ⟨x, hxS, hxV⟩ := h
+--   use x, hxS, x, hxS, Connected.refl hxV
+
+-- lemma symm (h : G.SetConnected S T) : G.SetConnected T S := by
+--   obtain ⟨s, hs, t, ht, h⟩ := h
+--   exact ⟨t, ht, s, hs, h.symm⟩
+
+-- lemma comm : G.SetConnected S T ↔ G.SetConnected T S := ⟨SetConnected.symm, SetConnected.symm⟩
+
+-- lemma left_subset (h : G.SetConnected S T) (hS : S ⊆ S') : G.SetConnected S' T := by
+--   obtain ⟨s, hs, t, ht, h⟩ := h
+--   use s, hS hs, t, ht
+
+-- lemma right_subset (h : G.SetConnected S T) (hT : T ⊆ T') : G.SetConnected S T' := by
+--   rw [SetConnected.comm] at h ⊢
+--   exact h.left_subset hT
+
+-- lemma subset (h : G.SetConnected S T) (hS : S ⊆ S') (hT : T ⊆ T') : G.SetConnected S' T' :=
+--   (h.left_subset hS).right_subset hT
+
+-- lemma left_supported : G.SetConnected S T ↔ G.SetConnected (S ∩ G.V) T := by
+--   constructor
+--   · rintro ⟨s, hsS, t, htT, h⟩
+--     use s, ⟨hsS, h.mem_left⟩, t, htT
+--   · rintro ⟨s, ⟨hsS, hs⟩, t, htT, h⟩
+--     use s, hsS, t, htT
+
+-- lemma right_supported : G.SetConnected S T ↔ G.SetConnected S (T ∩ G.V) := by
+--   rw [comm, left_supported, comm]
+
+-- lemma supported : G.SetConnected S T ↔ G.SetConnected (S ∩ G.V) (T ∩ G.V) := by
+--   rw [left_supported, right_supported]
+
+-- lemma le (h : G.SetConnected S T) (hle : G ≤ H) : H.SetConnected S T := by
+--   obtain ⟨s, hs, t, ht, h⟩ := h
+--   exact ⟨s, hs, t, ht, h.le hle⟩
+
+-- @[simp]
+-- lemma empty_source : ¬ G.SetConnected ∅ T := by
+--   rintro ⟨s, hs, t, ht, h⟩
+--   simp at hs
+
+-- @[simp]
+-- lemma empty_target : ¬ G.SetConnected S ∅ := by
+--   rw [SetConnected.comm]
+--   exact empty_source
+
+-- @[simp]
+-- lemma nonempty_inter (h : (S ∩ T ∩ G.V).Nonempty) : G.SetConnected S T := by
+--   obtain ⟨x, ⟨hxS, hxT⟩, hx⟩ := h
+--   use x, hxS, x, hxT, Connected.refl hx
+
+-- lemma exists_mem_left (h : G.SetConnected S T) : ∃ x ∈ S, x ∈ G.V := by
+--   obtain ⟨s, hs, t, ht, h⟩ := h
+--   exact ⟨s, hs, h.mem_left⟩
+
+-- lemma exists_mem_right (h : G.SetConnected S T) : ∃ x ∈ T, x ∈ G.V := by
+--   rw [SetConnected.comm] at h
+--   exact exists_mem_left h
+
+-- end SetConnected
