Matroid/ForMathlib/Graph/Subgraph.lean
@@ -1,0 +1,33 @@
+import Matroid.ForMathlib.Graph.Basic
+
+variable {α β : Type*} {x y z u v w : α} {e f : β} {G H : Graph α β}
+
+namespace Graph
+
+structure IsSubgraph (H G : Graph α β) : Prop where
+  vx_subset : H.V ⊆ G.V
+  inc₂_of_inc₂ : ∀ e x y, H.Inc₂ e x y → G.Inc₂ e x y
+
+/-- The subgraph order -/
+instance : PartialOrder (Graph α β) where
+  le := IsSubgraph
+  le_refl _ := ⟨rfl.le, by simp⟩
+  le_trans _ _ _ h₁ h₂ := ⟨h₁.1.trans h₂.1, fun _ _ _ h ↦ h₂.2 _ _ _ (h₁.2 _ _ _ h)⟩
+  le_antisymm G H h₁ h₂ := Graph.ext (h₁.1.antisymm h₂.1) fun e x y ↦ ⟨h₁.2 e x y, h₂.2 e x y⟩
+
+lemma Inc₂.of_le (h : H.Inc₂ e x y) (hle : H ≤ G) : G.Inc₂ e x y :=
+  hle.2 _ _ _ h
+
+lemma Inc.of_le (h : H.Inc e x) (hle : H ≤ G) : G.Inc e x :=
+  (h.choose_spec.of_le hle).inc_left
+
+lemma Adj.of_le (h : H.Adj x y) (hle : H ≤ G) : G.Adj x y :=
+  (h.choose_spec.of_le hle).adj
+
+lemma vxSet_subset_of_le (h : H ≤ G) : H.V ⊆ G.V :=
+  h.1
+
+lemma edgeSet_subset_of_le (h : H ≤ G) : H.E ⊆ G.E := by
+  refine fun e he ↦ ?_
+  obtain ⟨x, y, h'⟩ := exists_inc₂_of_mem_edgeSet he
+  exact (h'.of_le h).edge_mem
