Matroid/ForMathlib/Graph/Tree.lean
@@ -1,0 +1,4 @@
+import Matroid.ForMathlib.Graph.Connected
+
+variable {α β : Type*} {G H : Graph α β} {u v x y z : α} {e e' f g : β} {S S' T T' U V : Set α}
+  {F F' R R': Set β}
